# baseURI: http://publications.europa.eu/ontology/euvoc/linguisticDescriptions
# prefix: linguisticDescriptions

@prefix : <http://publications.europa.eu/ontology/euvoc/linguisticDescriptions#> .
@prefix dct: <http://purl.org/dc/terms/> .
@prefix euvoc: <http://publications.europa.eu/ontology/euvoc#> .
@prefix owl: <http://www.w3.org/2002/07/owl#> .
@prefix rdf: <http://www.w3.org/1999/02/22-rdf-syntax-ns#> .
@prefix rdfs: <http://www.w3.org/2000/01/rdf-schema#> .
@prefix skos: <http://www.w3.org/2004/02/skos/core#> .
@prefix skosxl: <http://www.w3.org/2008/05/skos-xl#> .
@prefix xsd: <http://www.w3.org/2001/XMLSchema#> .


<http://publications.europa.eu/ontology/euvoc/linguisticDescriptions>
  rdf:type owl:Ontology ;
  rdfs:comment "The EuVoc module importing and defining the linguistic relations and classes used in MDR authority tables"^^xsd:string ;
  rdfs:label "Linguistic Descriptions"^^xsd:string ;  
.

euvoc:XlNotation
  a owl:Class ;
  rdfs:comment "Current value and historical values of skos:notation."@en ;
  rdfs:label "Notation (reified SKOS notation)" ;  
.

euvoc:XlNote
  a owl:Class ;
  rdfs:comment "Current value and historical values of skos:note"@en ;
  rdfs:label "Note (reified SKOS note)" ;
.

euvoc:context
  a owl:ObjectProperty ;
  rdfs:comment "context" ;
  rdfs:label "context" ;
  skos:prefLabel "context" ;
.

euvoc:domain
  a owl:ObjectProperty ;
  rdfs:comment "To indicate the subject of the controlled vocabulary based on the Domain vocabulary, part of EuroVoc"@en ;
  rdfs:domain skos:ConceptScheme ;  
.

euvoc:order
  a owl:DatatypeProperty ;
  rdfs:comment "Current value of the order of the resource among its siblings"@en ;
  rdfs:range xsd:integer ;
.


euvoc:status
  a owl:ObjectProperty ;
  rdfs:comment "Indicates the status of a skos:Concept or a skosxl:Label, or any resource related to controlled vocabulary management."@en ;
  rdfs:range euvoc:ConceptStatus ;
.

euvoc:xlChangeNote
  a owl:ObjectProperty ;
  rdfs:comment "This property is a reified version of the skos:changeNote" ;
  rdfs:label "xl change note" ;
  rdfs:range euvoc:XlNote ;
  rdfs:subPropertyOf euvoc:xlNote ;
  skos:prefLabel "xl change note" ;
.



euvoc:xlDefinition
  a owl:ObjectProperty ;
  rdfs:comment "Relates a resource to the current and historical values of a skos:note."@en ;
  rdfs:range euvoc:XlNote ;
  rdfs:subPropertyOf euvoc:xlNote ;
.
euvoc:xlEditorialNote
  a owl:ObjectProperty ;
  rdfs:comment "This property is a reified version of the skos:editorialNote" ;
  rdfs:label "xl editorial note" ;
  rdfs:range euvoc:XlNote ;
  rdfs:subPropertyOf euvoc:xlNote ;
  skos:prefLabel "xl editorial note" ;
.

euvoc:xlHistoryNote
  a owl:ObjectProperty ;
  rdfs:comment "This property is a reified version of the skos:historyNote" ;
  rdfs:label "xl history note" ;
  rdfs:range euvoc:XlNote ;
  rdfs:subPropertyOf euvoc:xlNote ;
  skos:prefLabel "xl history note" ;
.
euvoc:xlNotation
  a owl:ObjectProperty ;
  rdfs:comment "Relates a resource to a Notation value."@en ;
  rdfs:range euvoc:XlNotation ;
.
euvoc:xlNote
  a owl:ObjectProperty ;
  rdfs:comment "This property is used to indicates the current and historical value of a note, for example a skos:note"@en ;
  rdfs:range euvoc:XlNote ;
.


euvoc:xlScopeNote
  a owl:ObjectProperty ;
  rdfs:comment "This property is a reified version of the skos:scopeNote" ;
  rdfs:label "xl scope note" ;
  rdfs:range euvoc:XlNote ;
  rdfs:subPropertyOf euvoc:xlNote ;
  skos:prefLabel "xl scope note" ;
.